$$
\vec x_0, \vec x_1,t_s,v,a_{acc},a_{dec}
$$

$$
\begin{aligned}
\vec x&= \vec x_1- \vec x_0\\
t_{acc} &= \frac{v}{a_{acc}}\\
t_{dec} &= \frac{v}{a_{dec}}\\
t_v&=\left(\vert x\vert-\frac{v^2}{2a_{acc}}-\frac{v^2}{2a_{dec}}\right)/v
\end{aligned}
$$

$$
t:=t_{acc}+t_{v}+t_{dec}
$$

$$
N=\frac{t}{t_s}
$$

$$
N_{acc;end} = N\frac{t_{acc}}{t};\quad N_{dec;begin} = N(1-\frac{t_{dec}}{t})
$$

$$
n=1,2,\cdots,N
$$

$$
\vec k = \frac{\vec x}{\vert x\vert}
$$

$$
\vec x(n) = \left\{\begin{aligned}
&\vec x(0) + \dfrac{1}{2}\vec k a_{acc}(nt_s)^2&&0<n<N_{acc}\\
&\vec x(0) + \dfrac{1}{2}\vec k a_{acc}(N_{acc}t_s)^2 + \vec k v(nt_s-t_{acc})&&N_{acc}<n<N_{dec}\\
&\vec x(0) + \dfrac{1}{2}\vec k a_{acc}(N_{acc}t_s)^2 + \vec k v(N_{dec}t_s-t_{acc}) + v\vec k(nt_s-N_{dec}t_s) - \frac{1}{2}\vec k a_{dec}(nt_s-N_{dec}t_s)^2 &&N_{dec}<n<N
\end{aligned}\right.
$$

$$
\vec x(n+1)- \vec x(n) = \left\{\begin{aligned}
&\dfrac{1}{2} a_{acc} \vec k t_s^2(2n+1)&&0<n<N_{acc}\\
&v\vec kt_s&&N_{acc}<n<N_{dec}\\
&v \vec k t_s-\frac{1}{2} a_{dec} \vec k t_s^2(2n+1-2N_{dec})  &&N_{dec}<n<N
\end{aligned}\right.
$$



